Sketching shallow wpp.
The downside of this is that it will be more difficult to set
up with the call rule. In that case, we want existential quantifiers
rather than universal ones. Generic automation might be able to address
that though.

theories/lang/cpp/logic/spec.v
@@ -29,51 +29,58 @@ Import ChargeNotation.
 Section with_prop.
   Context {PROP : bi}.
 
-  Record WithExG@{X Z Y R} {RESULT : Type@{R}} : Type :=
-    { we_ex   : tele@{X}
-    ; we_post : tele_fun@{X Z Y} we_ex (RESULT * PROP) }.
+  Definition WithExG@{R} {RESULT : Type@{R}} :=
+    (RESULT -> PROP) -> PROP.
   Global Arguments WithExG : clear implicits.
 
-  Definition WithExG_map@{X Z Y T U} {T : Type@{T}} {U : Type@{U}} (f : T -> PROP -> U * PROP)
-    (we : WithExG@{X Z Y T} T) : WithExG@{X Z Y U} U :=
-    {| we_ex := we.(we_ex)
-     ; we_post := tele_map (fun '(r,Q) => f r Q) we.(we_post) |}.
-
+  Definition WithPrePostG@{A R}  {ARGS : Type@{A}} {RESULT : Type@{R}} :=
+    ARGS -> (RESULT -> PROP) -> PROP.
+(*
   Record WithPrePostG@{X Z Y A R} {ARGS : Type@{A}} {RESULT : Type@{R}} :=
     { wpp_with : tele@{X}
     ; wpp_pre  : tele_fun@{X Z Y} wpp_with (ARGS * PROP)
-    ; wpp_post : tele_fun@{X Z Y} wpp_with (WithExG@{X Z _ _} RESULT)}.
+    ; wpp_post : tele_fun@{X Z Y} wpp_with (WithExG@{_} RESULT)}.
   Global Arguments WithPrePostG : clear implicits.
+ *)
 
   (** Mnemonic: WppGD stands for "[WithPrePostG]'s denotation" *)
-  Definition WppGD@{X Z Y A R} {ARGS RESULT} (wpp : WithPrePostG@{X Z Y A R} ARGS RESULT) (params : ARGS)
+  Definition WppGD@{A R} {ARGS RESULT} (wpp : @WithPrePostG@{A R} ARGS RESULT) (params : ARGS)
              (Q : RESULT -> PROP) : PROP :=
+    wpp params Q.
+  (*
+  refine (
     tbi_exist@{X Z Y} (tele_bind (TT:=wpp.(wpp_with)) (fun args =>
       let P := tele_app wpp.(wpp_pre) args in
-      let Q' := tele_app wpp.(wpp_post) args in
-      [| params = fst P |] ** snd P **
+      [| params = fst P |] ** snd P ** tele_app wpp.(wpp_post) args Q))).
+  Show Proof.
+
+
+  apply Q'. apply Q.
+  Show Proof.
       tbi_forall@{X Z Y} (tele_map (fun '(result,Q') => Q' -* Q result) Q'.(we_post)))).
+ *)
 
   (* Aliases specialized to [val]. We use definitions to control the universe
   arguments. *)
-  Definition WithEx@{X Z Y} := WithExG@{X Z Y _} val.
-  Definition WithPrePost@{X Z Y} := WithPrePostG@{X Z Y _ _} (list val) val.
-  Definition WppD@{X Z Y} := (WppGD@{X Z Y _ _} (ARGS := list val) (RESULT := val)).
-  Definition WithEx_map@{X Z Y} := WithExG_map@{X Z Y _ _} (T := val) (U := val).
+  Definition WithEx := WithExG@{Set} val.
+  Definition WithPrePost := @WithPrePostG@{Set Set} (list val) val.
+  Definition WppD := (WppGD (ARGS:=list val) (RESULT:=val)).
+(*  Definition WithEx_map@{X Z Y} := WithExG_map@{X Z Y _ _} (T := val) (U := val). *)
 End with_prop.
 
 Arguments WithPrePostG : clear implicits.
 Arguments WithPrePost : clear implicits.
-Arguments Build_WithPrePostG _ _ _ : clear implicits.
+(*Arguments Build_WithPrePostG _ _ _ : clear implicits. *)
 Arguments WithExG : clear implicits.
 Arguments WithEx : clear implicits.
-Arguments Build_WithExG _ _ _ : clear implicits.
+(*Arguments Build_WithExG _ _ _ : clear implicits. *)
 
-Arguments we_ex {PROP RESULT} _ : assert.
+(*Arguments we_ex {PROP RESULT} _ : assert.
 Arguments we_post {PROP RESULT} _ : assert.
 Arguments wpp_with {PROP ARGS RESULT} _: assert.
 Arguments wpp_pre {PROP ARGS RESULT} _: assert.
 Arguments wpp_post {PROP ARGS RESULT} _: assert.
+ *)
 
 Global Arguments WppGD {PROP ARGS RESULT} !wpp _ _ / : assert.
 Global Arguments WppD {PROP} !wpp _ _ / : assert.
@@ -98,6 +105,7 @@ End wpp_ofe.
 Arguments WithPrePostGO : clear implicits.
 Notation WithPrePostO PROP := (WithPrePostGO PROP (list val) val).
 
+(** TODO port this
 (** Universe polymorphic relations between WPPs. *)
 Definition wppg_relation@{X1 X2 Z1 Z2 Y1 Y2 A R} {PROP : bi} (R : relation PROP)
     {ARGS : Type@{A}} {RESULT : Type@{R}}
@@ -178,3 +186,4 @@ Section wpp_relations.
   Proof. apply wppg_dist_entailsN. Qed.
 
 End wpp_relations.
+*)
